James C - finally completed assembler

FiniteMap.thy
@@ -8,4 +8,8 @@ fun lookup :: "'a \<leadsto> 'b \<Rightarrow> 'a \<rightharpoonup> 'b" where
   "lookup [] k = None"
 | "lookup ((a, b) # ab) k = (if a = k then Some b else lookup ab k)"
 
+fun domain_distinct :: "'a \<leadsto> 'b \<Rightarrow> bool" where
+  "domain_distinct [] = True"
+| "domain_distinct ((a, b) # ab) = (domain_distinct ab \<and> a \<notin> dom (lookup ab))"
+
 end
